debug compilation OOM: Admitted pipeline_assumptions should have been in Prop, not in Type

compiler/src/examples/lightbulb.v
@@ -59,7 +59,13 @@ Instance mapops: RegAlloc.map.ops (SortedListString.map Z) :=
    (stack_pastend-4), next stack word to (stack_pastend-8) etc *)
 Definition stack_pastend: Z := 1024.
 Definition compile '(functions, initial, reactive) :=
-  compile_prog (p:=params) (RegAlloc.map.putmany_of_tuples map.empty functions) stack_pastend initial reactive (List.map fst functions).
+  compile_prog (p:=params) stack_pastend
+     (@Build_Program (FlattenExpr.mk_Semantics_params (@Pipeline.FlattenExpr_parameters params))
+                     (List.map fst functions)
+                     (RegAlloc.map.putmany_of_tuples map.empty functions)
+                     initial
+                     reactive).
+
 Definition instrencode p : list byte :=
   let word8s := List.flat_map (fun inst => HList.tuple.to_list (LittleEndian.split 4 (encode inst))) p in
   List.map (fun w => Byte.of_Z (word.unsigned w)) word8s.
@@ -69,14 +75,79 @@ Definition prog := (
   @cmd.skip flatparams,
   @cmd.call flatparams [] "iot" []).
 
-
+(*
 Import riscv.Utility.InstructionNotations.
 Import bedrock2.Hexdump.
 Local Open Scope hexdump_scope.
 Set Printing Width 108.
+*)
+
+Goal compile prog = nil.
+  cbv [compile compile_prog functions2Riscv prog].
+  match goal with
+  | |- context [@flatten_functions ?p ?E ?Fs] =>
+    let r := eval cbv in (@flatten_functions p E Fs) in change (@flatten_functions p E Fs) with r
+  end.
+  cbv [RegAlloc.rename_functions funnames List.map fst].
+  cbv [iot lightbulb recvEthernet].
+
+  match goal with
+  | |- context [RegAlloc.rename_function string Register funname string available_registers ?E ?N] =>
+    assert (RegAlloc.rename_function string Register funname string available_registers E N = (nil, nil, FlatImp.SSkip))
+  end.
+  {
+    unfold RegAlloc.rename_function.
+    match goal with
+    | |- context [@map.get ?k ?v ?m ?K ?M] =>
+      let r := eval cbv in (@map.get k v m K M) in change (@map.get k v m K M) with r
+    end.
+    cbv iota beta.
+    unfold RegAlloc.rename_fun.
+    simpl (RegAlloc.rename_binds string Register ["rx_packet"] available_registers).
+    cbv iota beta.
+    simpl (RegAlloc.rename_binds string Register ["r"]
+        [4; 5; 6; 7; 8; 9; 10; 11; 12; 13; 14; 15; 16; 17; 18; 19; 20; 21; 22; 23; 24; 25; 26;
+        27; 28; 29; 30; 31; 32; 33; 34; 35; 36; 37; 38; 39; 40; 41; 42; 43; 44; 45; 46; 47; 48;
+        49; 50; 51; 52]).
+    cbv iota beta.
+    cbv [RegAlloc.rename_stmt].
+    match goal with
+    | |- context [RegAlloc.rename string Register funname string ?A ?B ?C] =>
+      let r := eval cbv in (RegAlloc.rename string Register funname string A B C) in
+          change (RegAlloc.rename string Register funname string A B C) with r
+    end.
+    Set Printing Depth 100000.
+    cbv iota beta.
+    match goal with
+    | |- context [@RegAlloc.checker ?srcvar ?impvar ?func ?act ?src2imp ?ops ?m ?s] =>
+      set (test := ops)
+    end.
+    exfalso.
+
+    pose (m1 := map.put (map.put map.empty "a" 1) "b" 2).
+    pose (m2 := map.put (map.put map.empty "a" 1) "b" 22).
+    cbv in m1.
+    cbv in m2.
+    pose (m3 := RegAlloc.map.intersect m1 m2).
+    unfold RegAlloc.map.intersect, test, mapops in m3.
+    subst m1 m2.
+    assert (m3 = map.empty). {
+      subst test m3.
+      unfold ListLib.list_intersect.
+      simpl.
+      Set Printing Implicit.
+
+      (* culprit:
+@Pipeline.varname_eq_dec params pipeline_assumptions "a" "b"
+
+pipeline_assumptions is Admitted and lives in Type instead of Prop!
+       *)
+Abort.
+
+(*
 Goal True.
   Time
-  let r := eval cbv in (([[
+  let r := eval vm_compute in (([[
                          ]] ++ compile prog)%list%Z) in
   pose r as asm.
   (* {| value := [("iot", 0); ("lightbulb", 112); ("recvEthernet", 132)]; _value_ok := eq_refl |} *)
@@ -88,3 +159,4 @@ Goal True.
   let x := eval cbv in (instrencode asm) in
   idtac x.
 Abort.
+*)
